slight cleanups

examples/pseudo_bool/array/npbc_listScript.sml
@@ -1224,15 +1224,13 @@ QED
    No scoping and no proofgoals used *)
 Definition red_fast_def:
   red_fast s idopt pfs = (
-  if s = INR (Vector []) then
     case idopt of
       NONE => NONE
     | SOME id =>(
       case (pfs:scope) of
       | [(NONE,[(NONE,pf)])] => SOME (pf,id)
       | [] => SOME ([],id)
-      | _ => NONE)
-  else NONE)
+      | _ => NONE))
 End
 
 (* inds is just passed through here *)
@@ -1589,31 +1587,6 @@ Definition split_earliest_def:
 End
  *)
 
-(* A reverse mapping of vars -> indices *)
-Definition get_indices_def:
-  get_indices fml inds s (vimap:vimap_ty) =
-  case s of
-    INR v =>
-    if length v = 0 then []
-    else reindex fml inds
-  | INL (n,_) =>
-    case any_el n vimap NONE of
-      NONE => []
-    | SOME (INL (n,inds)) => reindex fml inds
-    | SOME (INR earliest) => reindex fml inds
-End
-
-(* We use a hard-coded limit on the reverse mapping, i.e.,
-  we store vars -> indices until the length of indices exceeds the limit.
-
-  however, we will ignore this limit for:
-  1. fresh variables that are introduced in a proof
-  2. any variable that is ever used in a witness (and we restore the mapping)
-*)
-Definition ind_lim_def:
-  ind_lim = 10n
-End
-
 Definition restore_aux_def:
   (restore_aux x fml [] iacc = REVERSE iacc) ∧
   (restore_aux x fml (i::is) iacc =
@@ -1630,8 +1603,33 @@ Definition restore_def:
   (restore x fml is = restore_aux x fml is [])
 End
 
+(* A reverse mapping of vars -> indices *)
+Definition get_indices_def:
+  get_indices fml inds s (vimap:vimap_ty) =
+  case s of
+    INR v =>
+    if length v = 0 then []
+    else reindex fml inds
+  | INL (n,_) =>
+    case any_el n vimap NONE of
+      NONE => []
+    | SOME (INL (n,inds)) => reindex fml inds
+    | SOME (INR earliest) => restore n fml inds
+End
+
+(* We use a hard-coded limit on the reverse mapping, i.e.,
+  we store vars -> indices until the length of indices exceeds the limit.
+
+  however, we will ignore this limit for:
+  1. fresh variables that are introduced in a proof
+  2. any variable that is ever used in a witness (and we restore the mapping)
+*)
+Definition ind_lim_def:
+  ind_lim = 10n
+End
+
 Definition set_indices_def:
-  set_indices fml inds s (vimap:vimap_ty) rinds =
+  set_indices inds s (vimap:vimap_ty) rinds =
   case s of
     INR v =>
     if length v = 0 then (inds,vimap)
@@ -1640,7 +1638,7 @@ Definition set_indices_def:
     case any_el n vimap NONE of
     | NONE => (inds,vimap)
     | SOME (INL _) => (inds , update_resize vimap NONE (SOME (INL (NONE ,rinds))) n)
-    | SOME (INR _) => (rinds, update_resize vimap NONE (SOME (INL (NONE ,restore n fml rinds))) n)
+    | SOME (INR _) => (inds, update_resize vimap NONE (SOME (INL (NONE ,rinds))) n)
 End
 
 Definition check_fresh_aux_fml_vimap_def:
@@ -1673,7 +1671,7 @@ Definition check_red_list_def:
   case red_fast ss idopt pfs of
     NONE => (
     let rinds = get_indices fml inds ss vimap in
-    let (inds',vimap') = set_indices fml inds ss vimap rinds in
+    let (inds',vimap') = set_indices inds ss vimap rinds in
     let nc = not c in
     let fml_not_c = update_resize fml NONE (SOME (nc,b)) id in
     let hs = has_scope pfs in
@@ -2574,6 +2572,27 @@ Proof
   every_case_tac>>fs[mk_subst_def]
 QED
 
+Theorem restore_aux:
+  ∀inds iacc.
+  restore_aux x fmlls inds iacc =
+  let is = FILTER (λn.
+    case any_el n fmlls NONE of NONE => F
+    | SOME c => MEM x (MAP SND (FST (FST c)))) inds in
+  (REVERSE iacc ++ is)
+Proof
+  Induct>>rw[restore_aux_def]>>
+  gvs[lookup_core_only_list_def,AllCaseEqs(),AllCasePreds()]>>
+  metis_tac[option_CLAUSES]
+QED
+
+Theorem restore_characterize:
+  restore x fmlls inds = FILTER (λn.
+    case any_el n fmlls NONE of NONE => F
+    | SOME c => MEM x (MAP SND (FST (FST c)))) inds
+Proof
+  rw[restore_def,restore_aux]
+QED
+
 Theorem MEM_get_indices_mk_subst:
   vimap_rel fmlls vimap ∧
   ind_rel fmlls inds ∧
@@ -2592,7 +2611,8 @@ Proof
     simp[]>>
     disch_then drule>>rw[]>>
     every_case_tac>>
-    gvs[reindex_characterize,MEM_FILTER,IS_SOME_EXISTS,ind_rel_def,PULL_EXISTS,any_el_ALT])
+    gvs[restore_characterize,reindex_characterize,MEM_FILTER,IS_SOME_EXISTS,ind_rel_def,PULL_EXISTS,any_el_ALT]
+    )
   >- (
     drule IS_SOME_subst_opt>>
     strip_tac>>
@@ -2619,7 +2639,7 @@ QED
 
 Theorem ind_rel_get_indices_set_indices:
   get_indices fmlls inds s vimap = rinds ∧
-  set_indices fmlls inds s vimap rinds = (inds',vimap') ∧
+  set_indices inds s vimap rinds = (inds',vimap') ∧
   ind_rel fmlls inds ⇒
   ind_rel fmlls inds'
 Proof
@@ -2628,29 +2648,8 @@ Proof
   metis_tac[ind_rel_reindex]
 QED
 
-Theorem restore_aux:
-  ∀inds iacc.
-  restore_aux x fmlls inds iacc =
-  let is = FILTER (λn.
-    case any_el n fmlls NONE of NONE => F
-    | SOME c => MEM x (MAP SND (FST (FST c)))) inds in
-  (REVERSE iacc ++ is)
-Proof
-  Induct>>rw[restore_aux_def]>>
-  gvs[lookup_core_only_list_def,AllCaseEqs(),AllCasePreds()]>>
-  metis_tac[option_CLAUSES]
-QED
-
-Theorem restore_characterize:
-  restore x fmlls inds = FILTER (λn.
-    case any_el n fmlls NONE of NONE => F
-    | SOME c => MEM x (MAP SND (FST (FST c)))) inds
-Proof
-  rw[restore_def,restore_aux]
-QED
-
 Theorem vimap_rel_get_indices_set_indices:
-  set_indices fmlls inds s vimap
+  set_indices inds s vimap
     (get_indices fmlls inds s vimap) = (inds',vimap') ∧
   vimap_rel fmlls vimap ∧
   ind_rel fmlls inds ⇒
